Switched LKSIZE to 8, generalized the proofs to accommodate; still some work to do on this.

concurrency/lksize.v
@@ -2,8 +2,6 @@ Require Import compcert.common.AST.
 Require Import compcert.common.Memdata.
 Require Import Coq.ZArith.ZArith.
 
-(* LKSIZE should be of the size of the struct we use for locks, which
-is sometimes equivalent to an array of 4 pointers. For now, we keep it
-equal to 1 (i.e. 4 bytes), but ideally it would be arbitrary. *)
-Definition LKSIZE:= 4%Z.
+(* LKSIZE should match sizeof(semax_conc.tlock).  *)
+Definition LKSIZE:= 8%Z.
 Definition LKSIZE_nat:= Z.to_nat LKSIZE.
