concurrency/semax_safety_freelock.v
@@ -275,15 +275,15 @@ Proof.
   apply (lock_inv_rmap_freelock CS) with (m := m) in Hlockinv; auto; try apply lock_coh.
   destruct Hlockinv as (phi0lockinv' & Hrmap00 & Hlkat).
 
-  assert (Hpos'' : (0 < 4)%Z) by omega.
-  pose proof rmap_freelock_join _ _ _ _ _ _ _ _ Hpos'' Hrmap00 jphi0 as Hrmap0.
+(*  assert (Hpos'' : (0 < 4)%Z) by omega. *)
+  pose proof rmap_freelock_join _ _ _ _ _ _ _ _ Hpos Hrmap00 jphi0 as Hrmap0.
   destruct Hrmap0 as (phi0' & Hrmap0 & jphi0').
-  pose proof rmap_freelock_join _ _ _ _ _ _ _ _ Hpos'' Hrmap0 Join as Hrmap.
+  pose proof rmap_freelock_join _ _ _ _ _ _ _ _ Hpos Hrmap0 Join as Hrmap.
   pose proof Hrmap as Hrmap_.
   destruct Hrmap_ as (phi' & RLphi & j').
   assert (ji : join_sub (getThreadR _ _ cnti) Phi) by join_sub_tac.
   destruct ji as (psi & jpsi). cleanup.
-  pose proof rmap_freelock_join _ _ _ _ _ _ _ _ Hpos'' RLphi jpsi as Hrmap'.
+  pose proof rmap_freelock_join _ _ _ _ _ _ _ _ Hpos RLphi jpsi as Hrmap'.
   destruct Hrmap' as (Phi' & Hrmap' & J').
 
   subst args.
@@ -360,7 +360,7 @@ Proof.
       rewrite <-joinlist_merge in j. 2: apply jphi0.
       rewrite joinlist_swap.
       destruct j as (xi_ & jxi_ & jx1).
-      pose proof rmap_freelock_join _ _ _ _ _ _ _ _ Hpos'' Hrmap00 jx1 as Hrmap1.
+      pose proof rmap_freelock_join _ _ _ _ _ _ _ _ Hpos Hrmap00 jx1 as Hrmap1.
       destruct Hrmap1 as (Phi'_ & Hrmap'_ & J).
       assert (Phi'_ = Phi') by (eapply rmap_freelock_unique; eauto). subst Phi'_.
       exists xi_. auto.
@@ -388,7 +388,7 @@ Proof.
         exact_eq M. f_equal.
         destruct Hrmap' as (_ & Same & Changed).
         spec Same loc. spec Changed loc.
-        destruct (adr_range_dec (b, Int.unsigned ofs) (4 * 1) loc) as [r|nr].
+        destruct (adr_range_dec (b, Int.unsigned ofs) LKSIZE loc) as [r|nr].
         -- autospec Changed.
            destruct Changed as (sh'' & rsh'' & ? & ? & ?).
            rewrite H,H1.
@@ -464,7 +464,7 @@ Proof.
       * discriminate.
       * intro IS; spec J IS.
         destruct Hrmap' as (_ & outside & inside). spec inside loc. spec outside loc.
-        destruct (adr_range_dec (b, Int.unsigned ofs) 4 loc).
+        destruct (adr_range_dec (b, Int.unsigned ofs) LKSIZE loc).
         -- autospec inside. exfalso.
            if_tac in inside; breakhyps.
         -- autospec outside. rewrite outside in J.
@@ -510,7 +510,7 @@ Proof.
         spec sparse loc (b, Int.intval ofs). rewrite locked in sparse. rewrite Eo in sparse.
         spec sparse. congruence.
         spec sparse. congruence.
-        destruct sparse as [ | sparse]. congruence.
+        destruct sparse as [ | sparse]. congruence. simpl in sparse.
         assert (SparseX: forall x, adr_range loc LKSIZE x -> ~adr_range (b, Int.unsigned ofs) 4 x).
         {
           clear -H sparse. intros x r.
@@ -529,7 +529,7 @@ Proof.
         destruct lock_coh_ as (LOAD & align & bound & R & lk & [sat | ?]). 2:omega.
         split; [ | split; [ | split ]]; auto.
         -- (* use sparsity to prove the load_at is the same *)
-           clear -LOAD SparseX locked.
+           clear -LOAD SparseX locked sparse.
            unfold load_at in *.
            destruct loc as (b0, ofs0); simpl in LOAD |- *.
            Transparent Mem.load.
@@ -560,15 +560,33 @@ Proof.
               if_tac [r|nr] in v1. 2:assumption.
               exfalso.
               spec SparseX' (b0, ofs1). spec SparseX'. split; auto; lkomega.
-              tauto.
-
+              destruct r; subst b0. simpl in sparse.
+              destruct sparse. contradiction H; auto. destruct H as [_ sparse].
+              red in sparse.
+              clear - SparseX SparseX' H0 r1 sparse. simpl in *.
+              change Int.intval with Int.unsigned in *.
+              assert (~ (Int.unsigned ofs <= ofs0 < Int.unsigned ofs + 4)%Z) 
+                      by (contradict SparseX; auto).
+              assert (~ (Int.unsigned ofs <= ofs1 < Int.unsigned ofs + 4)%Z)
+                      by (contradict SparseX'; auto).
+              clear - r1 H0 H H1 sparse. unfold LKSIZE in *.
+              forget (Int.unsigned ofs) as a.
+              assert (a+4 <= ofs1 < a+8)%Z by omega. clear H0 H1.
+              apply H; clear H. split ; try omega.
+              destruct (Zabs_dec (ofs0-a)); omega.
         -- exists R; split.
            ++ (* sparsity again, if easier or just the rmap_freelock *)
               intros x r.
               spec lk x r.
               destruct Hrmap' as (_ & outside & inside).
               spec outside x.
-              autospec outside.
+              spec outside. clear - sparse r.
+              destruct loc; destruct x; destruct r. subst b1.
+              intros [? ?]. subst b0. simpl in *. 
+              destruct sparse. contradiction H; auto. destruct H as [_ sparse].
+              change Int.intval with Int.unsigned in *.
+              red in sparse.
+              destruct (Zabs_dec (z - Int.unsigned ofs)); omega.
               rewrite age_to_resource_at.
               rewrite <-outside. clear outside.
               unfold sync_preds_defs.pack_res_inv in *.
@@ -606,7 +624,7 @@ Proof.
         destruct lock_coh_ as (LOAD & align & bound & R & lk).
         split; [ | split; [ | split ]]; auto.
         -- (* use sparsity to prove the load_at is the same *)
-           clear -LOAD SparseX locked.
+           clear -LOAD SparseX locked sparse.
            unfold load_at in *.
            destruct loc as (b0, ofs0); simpl in LOAD |- *.
            unfold Mem.load in *.
@@ -637,15 +655,33 @@ Proof.
               if_tac [r|nr] in v1. 2:assumption.
               exfalso.
               spec SparseX' (b0, ofs1). spec SparseX'. split; auto; lkomega.
-              tauto.
-
+              simpl in sparse. 
+              destruct r; subst b0.
+              clear - SparseX SparseX' H0 r1 sparse. simpl in *.
+              destruct sparse. contradiction H; auto. destruct H as [_ sparse].
+              change Int.intval with Int.unsigned in *.
+              assert (~ (Int.unsigned ofs <= ofs0 < Int.unsigned ofs + 4)%Z) 
+                      by (contradict SparseX; auto).
+              assert (~ (Int.unsigned ofs <= ofs1 < Int.unsigned ofs + 4)%Z)
+                      by (contradict SparseX'; auto).
+              clear - r1 H0 H H1 sparse. unfold LKSIZE in *.
+              forget (Int.unsigned ofs) as a.
+              assert (a+4 <= ofs1 < a+8)%Z by omega. clear H0 H1.
+              apply H; clear H. split ; try omega.
+              red in sparse; unfold LKSIZE in *; destruct (Zabs_dec (ofs0-a)); try omega.
         -- exists R.
            (* sparsity again, if easier or just the rmap_freelock *)
            intros x r.
            spec lk x r.
            destruct Hrmap' as (_ & outside & inside).
            spec outside x.
-           autospec outside.
+              spec outside. clear - sparse r.
+              destruct loc; destruct x; destruct r. subst b1.
+              intros [? ?]. subst b0. simpl in *. 
+              destruct sparse. contradiction H; auto. destruct H as [_ sparse].
+              change Int.intval with Int.unsigned in *.
+              red in sparse.
+              destruct (Zabs_dec (z - Int.unsigned ofs)); omega.
            rewrite age_to_resource_at.
            rewrite <-outside. clear outside.
            unfold sync_preds_defs.pack_res_inv in *.
@@ -740,7 +776,6 @@ Proof.
               split. now apply age_to_join; auto.
               split. 
               apply age_to_pred.
-              replace 2%Z with 1%Z by admit.   (* mismatch between LKSIZE=4 and LKSIZE=8 *)
               assumption.
               apply age_to_pred. assumption.
           + exact_eq Safe'.
@@ -779,4 +814,4 @@ Proof.
     eapply unique_Krun_no_Krun. eassumption.
     instantiate (1 := cnti). rewr (getThreadC i tp cnti).
     congruence.
-Admitted.
+Qed.
